theories/SSProve.v
@@ -325,3 +325,36 @@ Proof.
     - apply Cross_conj_left, Cross_conj_left, H1.
   + apply H2.
 Qed.
+
+
+Inductive NoFail {A} : raw_code A → Prop :=
+  | NoFail_ret : ∀ x,
+      NoFail (ret x)
+  | NoFail_sampler : ∀ op k,
+      LosslessOp op →
+      (∀ v, NoFail (k v)) →
+      NoFail (pkg_core_definition.sampler op k).
+
+Lemma r_NoFail_L {A B : choiceType} (c : raw_code B) (c₀ : B → raw_code A) (c₁ : raw_code A)
+    (pre : precond) (post : postcond A A) :
+    NoFail c →
+    (∀ x : B, ⊢ ⦃ pre ⦄ c₀ x ≈ c₁ ⦃ post ⦄) →
+    ⊢ ⦃ pre ⦄ x ← c ;; c₀ x ≈ c₁ ⦃ post ⦄.
+Proof.
+  intros H H'.
+  elim: H; intros.
+  + apply H'.
+  + by apply r_const_sample_L.
+Qed.
+
+Lemma r_NoFail_R {A B : choiceType} (c : raw_code B) (c₀ : raw_code A) (c₁ : B → raw_code A)
+    (pre : precond) (post : postcond A A) :
+    NoFail c →
+    (∀ x : B, ⊢ ⦃ pre ⦄ c₀ ≈ c₁ x ⦃ post ⦄) →
+    ⊢ ⦃ pre ⦄ c₀ ≈ x ← c ;; c₁ x ⦃ post ⦄.
+Proof.
+  intros H H'.
+  elim: H; intros.
+  + apply H'.
+  + by apply r_const_sample_R.
+Qed.
